Begin specifying call

iodiv/IODiv.fst
@@ -51,6 +51,9 @@ unfold
 let iopos = ipos cmds io_op_sig
 
 unfold
+let ionode = inode cmds io_op_sig
+
+unfold
 let iochoice = ichoice cmds io_op_sig
 
 unfold
@@ -427,11 +430,29 @@ let iodiv_tau #a #w (m : iodiv a w) : iodiv a w =
   assert (forall (post : wpost a). w post ==> theta (tau m) post) ;
   tau m
 
-// let wcall #a (o : cmds) (x : io_args o) (w : io_res o -> twp a) : twp a =
-//   fun post -> post [] None /\ (forall y. w y (shift_post [ Call_choice o x y ] post))
+let wcall #a (o : cmds) (x : io_args o) (w : io_res o -> twp a) : twp a =
+  fun post -> forall y. w y (shift_post [ Call_choice o x y ] post)
 
-// let iodiv_call #a (o : cmds) (x : io_args o) #w (k : (r : io_res o) -> iodiv a (w r)) : iodiv a (wcall o x w) =
-//   call o x k
+let isCall_choice (o : cmds) (x : io_args o) (t : iochoice) =
+  match t with
+  | Call_choice o' x' y -> o = o' && x = x'
+  | _ -> false
+
+let call_choice_res (o : cmds) (x : io_args o) (t : iochoice) :
+  Pure (io_res o) (requires isCall_choice o x t) (ensures fun _ -> True)
+= match t with
+  | Call_choice o' x' y -> y
+
+let iodiv_call #a (o : cmds) (x : io_args o) #w (k : (r : io_res o) -> iodiv a (w r)) : iodiv a (wcall o x w) =
+  // fin
+  assert (forall p. isRet (call o x k p) ==> isCall_choice o x (hd p) /\ isRet (k (call_choice_res o x (hd p)) (tl p))) ;
+  assume (forall (post : wpost a) p. wcall o x w post ==> isRet (call o x k p) ==> theta (call o x k) post) ;
+
+  // inf
+  assume (forall (post : wpost a) (p p' : iopostream). wcall o x w post ==> event_stream (call o x k) p ==> p `uptotau` p' ==> theta (call o x k) post) ;
+
+  assert (forall (post : wpost a). wcall o x w post ==> theta (call o x k) post) ;
+  call o x k
 
 // let rec wrepeat_trunc (w : twp unit) (n : nat) : twp unit =
 //   if n = 0
